WIP

src/TU_to_Core.v
@@ -1,6 +1,7 @@
 Require Import Common. 
 Require Core TaggedUnions. 
 Require Import PArith. 
+
 Module S := TaggedUnions.  
 Module T := Core. 
 
@@ -11,165 +12,26 @@ refine  (Finite.Build_T _ 0 _). simpl. admit.
 refine  (Finite.Build_T _ (S (Finite.val IHX)) _). simpl. admit.
 Defined.
 
-Class Ordered  (X : Type) := {compare : X -> X -> comparison}.  
-
-Local Notation lex e f := (match e with Eq => f | _ => e end).
-
-
-Module M. 
-  
-  Section t. 
-    Variable X : Type. 
-    Context {O : Ordered X}. 
-    
-    
-
-    Definition T := list (positive * X). 
-    
-    Definition singleton x : T := ([(1%positive,x)])%list. 
-    
-    Fixpoint add n x (l : T) : T :=
-      match l with 
-        | nil => [(n,x)]
-        | (m,y)::q => 
-            match compare x y with 
-              | Lt => (n, x) :: l
-              | Eq => (n+m,x)%positive :: q 
-              | Gt => (m,y):: add n x q
-            end
-      end%list. 
-
-    Fixpoint max n x (l : T) : T :=
-      match l with 
-        | nil => [(n,x)]
-        | (m,y)::q => 
-            match compare x y with 
-              | Lt => (n, x) :: l
-              | Eq => (Pos.max n m,x)%positive :: q 
-              | Gt => (m,y):: max n x q
-            end
-      end%list. 
-    
-    Fixpoint union (a b : T) : T :=
-      match a with 
-        |nil => b 
-        | (n,x) :: q => add n x (union q b)
-      end%list. 
-
-    Fixpoint join (a b : T) : T :=
-      match a with 
-        |nil => b 
-        | (n,x) :: q => max n x (join q b)
-      end%list. 
-    
-    Fixpoint copy n (x : X)  :=
-      match n with 
-        | xH => [x]
-        | xO m => copy m x ++ copy m x
-        | xI m => x :: copy m x  ++ copy m x
-      end%list. 
-
-    Fixpoint contents (a : T) := 
-      match a with 
-        | nil => nil
-        | (n,x) :: q => copy n x ++ (contents q)
-      end%list.         
-    
-    Fixpoint elements (a : T) : list X := List.map (@snd _ _) a. 
-    
-    Fixpoint of_list (l : list X) : T :=
-      match l with 
-        | nil => nil
-        | cons t q => add 1 t (of_list q)
-      end. 
-  End t. 
-  Arguments singleton {X} _. 
-  Arguments add {X _} n x l. 
-  Arguments union {X _} a b. 
-  Arguments join {X _} a b. 
-  Arguments of_list {X _} l.  
-
-End M. 
-
-Definition type0_cmp t t' := 
-  match t , t' with 
-    | Tunit, Tunit => Eq
-    | Tbool, Tbool => Eq
-    | Tint n , Tint m => NPeano.Nat.compare n m 
-    | Tfin n , Tfin m => NPeano.Nat.compare n m 
-
-    | Tunit, _ => Lt
-    | _, Tunit => Gt
-
-    | Tbool, _ => Lt
-    | _, Tbool => Gt
-
-    | Tint _, _ => Lt
-    | _, Tint _ => Gt
-
-    | Tfin _, _ => Lt
-    | _, Tfin _ => Gt       
-
-    | Tabstract _ _, _ => Lt
-  end. 
-
-Fixpoint type_cmp  t t' {struct t} :=
-  match t, t' with 
-      | T.Tlift t, T.Tlift t' => type0_cmp t t'
-      | T.Ttuple l, T.Ttuple l' => 
-          let list_compare := fix list_compare h k :=
-              match h,k with 
-                | nil, nil => Eq
-                | nil, _ => Lt
-                | _, nil => Gt
-                | cons t q, cons t' q' => lex (type_cmp t t') (list_compare q q')
-              end in 
-
-          list_compare l l' 
-      | T.Tlift _, _ => Lt
-      | _,  T.Tlift _ => Gt
-  end. 
-
 Section compile. 
   Variable Phi : S.state. 
   
 
-  Instance Ord : Ordered T.type. 
-  refine  (Build_Ordered _ type_cmp). 
-  Defined. 
-
-  Definition open (x :  T.type) : M.T T.type :=
+  Variable layout : list S.type -> list T.type.
+  Fixpoint scheme (x : S.type) : T.type :=
     match x with 
-      | T.Tlift t0 => M.singleton (T.Tlift t0)
-      | T.Ttuple l => M.of_list l
+        S.Tlift t => T.Tlift t
+      | S.Ttuple l => T.Ttuple (List.map scheme l)
+      | S.Tunion l => T.Ttuple (T.Tlift (Tfin (List.length l)) :: layout l)
     end. 
-
-  Definition process (l : list T.type) : M.T T.type :=
-    List.fold_right M.join []%list  (List.map open  l).  
-
   
-  Definition flat : S.type -> T.type .
-  intros x. 
-  refine (
-      let f := fix convert (x : S.type) : T.type :=
-          match x with 
-                  | S.Tlift t0 => T.Tlift t0
-                  | S.Ttuple l => T.Ttuple (List.map convert l)
-                  | S.Tunion C =>  
-                            let l := List.map convert C in 
-                            let m := process l in
-                            let c := T.Tlift (Tfin (List.length C )) in 
-                              T.Ttuple (c:: M.contents _ m)
-
-          end in _). 
-  apply (f x). 
-  Defined. 
+  Variable allocate : forall R t l (c : var l t) (x : T.expr R (scheme t)),  T.expr R (scheme (S.Tunion l)). 
+  Variable deallocate: forall R l t (c : var l t), T.expr R (scheme (S.Tunion l)) -> T.expr R (scheme t).
 
   Definition compile_sync : S.sync -> T.sync. 
   Proof. 
     refine (fun X => match X with
-                      |S.Treg t => T.Treg (flat t)
-                      |S.Tregfile n t => T.Tregfile n (flat t)
+                      |S.Treg t => T.Treg (scheme t)
+                      |S.Tregfile n t => T.Tregfile n (scheme t)
             end). 
   Defined. 
 
@@ -178,13 +40,11 @@ Section compile.
 
   Definition compile_state : S.state -> T.state := List.map compile_sync. 
 
-
-  Variable (R : T.type -> Type). 
   Definition A := S.Tlift Tbool. 
 
-  Eval compute in flat (S.Tunion [ S.Tunion [A;A]; A]). 
-  Eval compute in flat (S.Tunion [ S.Tunion [A;A]; S.Tunion [S.Ttuple [A ; A] ; A; A]]). 
-  Eval compute in flat (S.Tunion [ S.Tunion [A;A]; S.Tunion [A;A]; S.Tunion [S.Ttuple [A ; A] ; A; A]]). 
+  Eval compute in scheme (S.Tunion [ S.Tunion [A;A]; A]). 
+  Eval compute in scheme (S.Tunion [ S.Tunion [A;A]; S.Tunion [S.Ttuple [A ; A] ; A; A]]). 
+  Eval compute in scheme (S.Tunion [ S.Tunion [A;A]; S.Tunion [A;A]; S.Tunion [S.Ttuple [A ; A] ; A; A]]). 
 
   (** Allocate takes the constructor [c] applied to [x], and return
   the corresponding tuple. 
@@ -205,228 +65,401 @@ Section compile.
  *)
 
     
-    Definition Eapp l1 l2 : 
-      T.expr R (T.Ttuple l1) -> T.expr R (T.Ttuple l2) -> 
-      T.expr R (T.Ttuple (l1 ++ l2)).  
-    Admitted. 
-    Definition Eskip l1 l2 : 
-      T.expr R (T.Ttuple (l1 ++ l2)) -> T.expr R (T.Ttuple (l2)).  
-    Admitted. 
-    Definition Efirst l1 l2 : 
-      T.expr R (T.Ttuple (l1 ++ l2)) -> T.expr R (T.Ttuple (l1)).     
-    Admitted. 
+    (* Definition Eapp l1 l2 :  *)
+    (*   T.expr R (T.Ttuple l1) -> T.expr R (T.Ttuple l2) ->  *)
+    (*   T.expr R (T.Ttuple (l1 ++ l2)).   *)
+    (* Admitted.  *)
+    (* Definition Eskip l1 l2 :  *)
+    (*   T.expr R (T.Ttuple (l1 ++ l2)) -> T.expr R (T.Ttuple (l2)).   *)
+    (* Admitted.  *)
+    (* Definition Efirst l1 l2 :  *)
+    (*   T.expr R (T.Ttuple (l1 ++ l2)) -> T.expr R (T.Ttuple (l1)).      *)
+    (* Admitted.  *)
     
-    Definition Enull  t : T.expr R t. Admitted.  
+    (* Definition Enull  t : T.expr R t. Admitted.   *)
     
-    Definition Econs t l : 
-      T.expr R t -> T.expr R (T.Ttuple l) -> 
-      T.expr R (T.Ttuple (t::l)).  
-    Admitted. 
+    (* Definition Econs t l :  *)
+    (*   T.expr R t -> T.expr R (T.Ttuple l) ->  *)
+    (*   T.expr R (T.Ttuple (t::l)).   *)
+    (* Admitted.  *)
 
   Section t. 
-    Notation MS := (M.T T.type). 
+    (* Notation MS := (M.T T.type).  *)
 
+    
+    (* Definition type_eqb : T.type -> T.type -> bool. Admitted.  *)
+(*     Definition type_eqb_correct x y : type_eqb x y = true -> x = y. Admitted.  *)
+(*     Definition proj_on_t l t' (e : T.expr R (T.Ttuple l)) : list (T.expr R t').  *)
+(*     revert  t' e.  *)
+(*     induction l.  *)
+(*     intros. apply nil.  *)
+(*     intros. set (hd := T.Efst _ _ _ e).  *)
+(*     case_eq (type_eqb a  t'). intros. apply cons.  *)
+    
+(*     erewrite <- type_eqb_correct. apply hd. apply H.  *)
+(*     apply IHl. apply (T.Esnd _ _ _ e).  *)
+(*     intros. apply IHl. apply (T.Esnd _ _ _ e).  *)
+(*     Defined.  *)
+    
+(*     Definition zob (t : T.type) : list T.type.  *)
+(*     destruct t.  *)
+(*     refine ([T.Tlift t])%list.  *)
+(*     exact l.  *)
+(*     Defined.  *)
+    
+(*     Definition unpack t : T.expr R t -> T.expr R (T.Ttuple (zob t)). Admitted.  *)
 
-      Definition type_eqb : T.type -> T.type -> bool. Admitted. 
-      Definition type_eqb_correct x y : type_eqb x y = true -> x = y. Admitted. 
-    Definition proj_on_t l t' (e : T.expr R (T.Ttuple l)) : list (T.expr R t'). 
-    revert  t' e. 
-    induction l. 
-    intros. apply nil. 
-    intros. set (hd := T.Efst _ _ _ e). 
-    case_eq (type_eqb a  t'). intros. apply cons. 
-    
-    erewrite <- type_eqb_correct. apply hd. apply H. 
-    apply IHl. apply (T.Esnd _ _ _ e). 
-    intros. apply IHl. apply (T.Esnd _ _ _ e). 
-    Defined. 
-    
-    Definition zob (t : T.type) : list T.type. 
-    destruct t. 
-    refine ([T.Tlift t])%list. 
-    exact l. 
-    Defined. 
-    
-    Definition unpack t : T.expr R t -> T.expr R (T.Ttuple (zob t)). Admitted. 
-
-    Definition allocate t l (c : var l t) (x : T.expr R (flat t)) : T.expr R (flat (S.Tunion l)). 
-    Proof. 
-      simpl flat.
-      match goal with 
-          |- context [M.contents _ ?c] => set (ms := c)
-      end. 
-      set (types := M.elements _ ms). 
-      apply Econs. admit. 
-      refine (
-          let tutu := fix tutu l : T.expr _ (T.Ttuple (M.contents _ l)):= 
-              match l with 
-                | nil => T.Etuple  _ _ (DList.dlist_nil)
-                | (n,x) :: q => _
-              end%list in 
-            (tutu _)
-        ).
-      apply Eapp. 2: apply tutu. 
+(*     Definition allocate t l (c : var l t) (x : T.expr R (scheme t)) : T.expr R (scheme (S.Tunion l)).  *)
+(*     Proof.  *)
+(*       simpl scheme. *)
+(*       match goal with  *)
+(*           |- context [M.contents _ ?c] => set (ms := c) *)
+(*       end.  *)
+(*       set (types := M.elements _ ms).  *)
+(*       apply Econs. admit.  *)
+(*       refine ( *)
+(*           let tutu := fix tutu l : T.expr _ (T.Ttuple (M.contents _ l)):=  *)
+(*               match l with  *)
+(*                 | nil => T.Etuple  _ _ (DList.dlist_nil) *)
+(*                 | (n,x) :: q => _ *)
+(*               end%list in  *)
+(*             (tutu _) *)
+(*         ). *)
+(*       apply Eapp. 2: apply tutu.  *)
       
-    apply unpack in x. 
-    eapply proj_on_t in x. 
+(*     apply unpack in x.  *)
+(*     eapply proj_on_t in x.  *)
       
-      Definition pad n t : list (T.expr R t) -> T.expr R (T.Ttuple (M.copy _  n t)). Admitted. 
-   apply (pad _ _ x). 
+(*       Definition pad n t : list (T.expr R t) -> T.expr R (T.Ttuple (M.copy _  n t)). Admitted.  *)
+(*    apply (pad _ _ x).  *)
+(*     Defined.  *)
+
+(*     (* This function must cherry-pick the right types. It assumes that *)
+(*     the check that the tag is the right one was done elsewhere *) *)
+
+(*   Definition deallocate t l tr (c : var l t) (e : T.expr R (scheme (S.Tunion l)))  *)
+(*                         (cont : R (scheme t) -> T.action (compile_state Phi) R (scheme tr)):  *)
+(*     T.action (compile_state Phi) R (scheme tr).  *)
+(*   Proof.  *)
+(*     simpl in e.  *)
+(*     apply T.Esnd in e.  *)
+(*     eapply T.Bind.  *)
+(*     eapply T.Return. 2: apply cont. clear cont.  *)
+    
+(*     Definition test (t : T.type) : T.expr R (T.Ttuple (zob t)) -> T.expr R (t).  *)
+(*     destruct t.  simpl. apply T.Efst.  *)
+(*     simpl. apply id.  *)
+(*     Defined.  *)
+
+(*     apply test.  *)
+(* revert e.  *)
+(*       match goal with  *)
+(*           |- context [M.contents _ ?c] => set (ms := c) *)
+(*       end. *)
+      
+(*       Definition layout (E : list T.type) (L : list T.type) := DList.dlist (fun x => var L x) E.  *)
+
+      
+(*       Definition get_layout t l (c : var l t) : layout (zob t) (M.contents  _ (process l)). Admitted.  *)
+    
+(*     set (ohmy := get_layout  _ _ (var_map (scheme ) _ _ c)). *)
+
+(*     change (fun x : S.type => scheme x) with scheme in ms.  *)
+(*     fold ms in ohmy.  *)
+(*     clearbody ohmy. clearbody ms.  *)
+
+(*     induction ms. simpl in ohmy. unfold layout in *. simpl. admit.  *)
+(*     simpl in *.  *)
+(*     intros.  *)
+(*     destruct a.  *)
+ 
+(*     simpl.  *)
+(*     unfold ms in *.  *)
+(*       intros e.  *)
+(*       induction ms.  *)
+(*       simpl.  *)
+(*       refine ( *)
+
+(*           let tutu := fix tutu l : T.expr _ (T.Ttuple (M.contents _ l)):=  *)
+(*               match l with  *)
+(*                 | nil => T.Etuple  _ _ (DList.dlist_nil) *)
+(*                 | (n,x) :: q => _ *)
+(*               end%list in  *)
+(*             (tutu _) *)
+(*         ). *)
+
+(* REVERT E.  *)
+(*     refine ( *)
+(*         let tutu := fix tutu l : T.expr _ (T.Ttuple (M.contents _ l)):=  *)
+(*             match l with  *)
+(*               | nil => T.Etuple  _ _ (DList.dlist_nil) *)
+(*               | (n,x) :: q => _ *)
+(*             end%list in  *)
+(*           (tutu _) *)
+(*       ). *)
+
+    
+(*   Qed.      *)
+    
+  Section compile. 
+
+    Variable (R : T.type -> Type). 
+    
+    Definition compile_expr t : S.expr (fun x => R (scheme x)) t  -> T.expr R (scheme t).  
+    
+    refine (let compile := fix compile t (e : S.expr (fun x => R (scheme x)) t) : T.expr R (scheme t) := 
+                match e with
+                  | S.Evar t v => T.Evar v
+                  | S.Ebuiltin args res f x => 
+                      T.Ebuiltin f (DList.dlist_map (fun x X => compile _ X) args x)
+                  | S.Econstant ty c => T.Econstant c
+                  | S.Efst l t x => T.Efst _ _ _ (compile _ x)
+                  | S.Esnd l t x => T.Esnd _ _ _ (compile _ x)
+                  | S.Enth l t m x => T.Enth  (var_map _ _ _ m) (compile _ x) 
+                  | S.Etuple l exprs => T.Etuple _ _ (DList.dmap _ _ _ compile _ exprs)
+                  | S.Econstr l t c x => allocate R t l c (compile _ x)
+                end  
+            in compile t
+           ). 
     Defined. 
 
-    (* This function must cherry-pick the right types. It assumes that
-    the check that the tag is the right one was done elsewhere *)
+    
+    Definition compile   t : S.action Phi (fun x => R (scheme x )) t -> T.action (compile_state Phi ) R (scheme t). 
+    refine (let compile := fix compile t (a : S.action Phi (fun x => R (scheme x)) t) : 
+                           T.action (compile_state Phi) R (scheme t) :=
+                match a with
+                  | S.Return t exp => T.Return (compile_expr _ exp)
+                  | S.Bind t u a f => T.Bind (compile _ a) (fun X => compile _ (f X))  
+                  | S.Assert e => T.Assert (compile_expr _ e)
+                  | S.Primitive args res p exprs => 
+                      let exprs := 
+                          (DList.dmap (S.expr (fun x : S.type => R (scheme x))) 
+                                (T.expr R) scheme compile_expr args exprs)
+                      in 
+                        T.Primitive (List.map scheme args) (scheme res) _ exprs
+                  | S.Try a => T.Try _ _ (compile _ a)
+                  | S.Case td l t c e x => _
+                end
+            in compile t
+           ). 
+    (* primities *)
+    clear exprs0. revert exprs. 
+    refine (match p with 
+                S.register_read t v => fun exprs =>
+                                        (
+                                          T.register_read  (var_map compile_sync _ _ v)
+                                          :T.primitive (compile_state Phi) (List.map scheme []) (scheme t))
+                                          
+              | S.register_write t v => fun exprs => 
+                                         (
+                                           T.register_write (var_map compile_sync Phi (S.Treg t) v)
+                                           :T.primitive (compile_state Phi) (List.map scheme [t])
+                                             (scheme (S.Tlift Tunit))
+                                         )
+              | S.regfile_read n t v p => fun exprs => ( T.regfile_read
+                                                        (var_map compile_sync Phi (S.Tregfile n t) v) p
+                                                       :T.primitive (compile_state Phi)
+                                                       (List.map scheme [S.Tlift (W p)]) 
+                                                       (scheme t))
+              | S.regfile_write m t v p => fun exprs => 
 
-  Definition deallocate t l tr (c : var l t) (e : T.expr R (flat (S.Tunion l))) 
-                        (cont : R (flat t) -> T.action (compile_state Phi) R (flat tr)): 
-    T.action (compile_state Phi) R (flat tr). 
+                                            (   T.regfile_write
+                                                 (var_map compile_sync Phi (S.Tregfile m t) v) p
+                                                :T.primitive (compile_state Phi)
+                                                  (List.map scheme [S.Tlift (W p); t])
+                                                  (scheme (S.Tlift Tunit)))
+            end ). 
+    (* Case case *)
+    + idtac.      
+      apply compile_expr in e.
+      Import T. 
+      refine (WHEN (# (fin_of_var _ _ c : constant0 (Tfin _))  = Efst _ _ _ e ) ; 
+              DO R <- Return _ ; 
+              compile _ (x R)
+             ). 
+      
+
+      apply (deallocate R _ _ c e).  
+    Defined. 
+  End compile. 
+  
+  Definition Compile t (a : S.Action Phi t) : T.Action (compile_state Phi) (scheme t) := 
+    fun  _ => compile _ t (a _).  
+  
+  (* we start by defining what it means to be equivalent as values *)
+  
+  Notation " l & Gamma |- x == y" := (S.WF.equiv_action _ _ _ l Gamma _ x y) (no associativity, at level 80). 
+
+  Lemma correct l Gamma t a b R: 
+    l & Gamma |- a == b ->
+    R (@S.Sem.eval_action Phi t a) 
+      (@T.Sem.eval_action (compile_state Phi) (scheme t) (compile _ _ b)). 
   Proof. 
-    simpl in e. 
-    apply T.Esnd in e. 
-    eapply T.Bind. 
-    eapply T.Return. 2: apply cont. clear cont. 
+
+    Fixpoint tuple_eq {A} 
+                        (F : A -> Type )
+                        (G : A -> Type)
+                        (R : forall x, F x -> G x -> Prop)
+                        (l : list A) : Tuple.of_list F l ->  Tuple.of_list G l -> Prop :=
+      match l with 
+          | nil => fun _ _  => True
+          | cons t q => fun t1 t2 => R _ (Tuple.fst t1) (Tuple.fst t2) /\ 
+                                     tuple_eq F G R q (Tuple.snd t1)  (Tuple.snd t2)
+      end. 
     
-    Definition test (t : T.type) : T.expr R (T.Ttuple (zob t)) -> T.expr R (t). 
-    destruct t.  simpl. apply T.Efst. 
-    simpl. apply id. 
-    Defined. 
-
-    apply test. 
-revert e. 
-      match goal with 
-          |- context [M.contents _ ?c] => set (ms := c)
-      end.
-      
-      Definition layout (E : list T.type) (L : list T.type) := DList.dlist (fun x => var L x) E. 
-
-      
-      Definition get_layout t l (c : var l t) : layout (zob t) (M.contents  _ (process l)). Admitted. 
-    
-    set (ohmy := get_layout  _ _ (var_map (flat ) _ _ c)).
-
-    change (fun x : S.type => flat x) with flat in ms. 
-    fold ms in ohmy. 
-    clearbody ohmy. clearbody ms. 
-
-    induction ms. simpl in ohmy. unfold layout in *. simpl. admit. 
-    simpl in *. 
+    Definition equiv_sync t : S.eval_sync t -> T.eval_sync (compile_sync t) -> Prop. Admitted. 
+    Definition equiv_state l :  (S.eval_state l) -> (T.eval_state (compile_state l)) -> Prop.    
     intros. 
-    destruct a. 
- 
-    simpl. 
-    unfold ms in *. 
-      intros e. 
-      induction ms. 
-      simpl. 
-      refine (
+   eapply tuple_eq. apply equiv_sync. apply X. unfold T.eval_state in *. apply X0. 
+2: apply X. 
 
-          let tutu := fix tutu l : T.expr _ (T.Ttuple (M.contents _ l)):= 
-              match l with 
-                | nil => T.Etuple  _ _ (DList.dlist_nil)
-                | (n,x) :: q => _
-              end%list in 
-            (tutu _)
-        ).
 
-REVERT E. 
-    refine (
-        let tutu := fix tutu l : T.expr _ (T.Ttuple (M.contents _ l)):= 
-            match l with 
-              | nil => T.Etuple  _ _ (DList.dlist_nil)
-              | (n,x) :: q => _
-            end%list in 
-          (tutu _)
-      ).
+    2: apply X0. := tuple_eq _ _ _ l. 
+                                                                              
+  S.eval_state   
+ (* R : S.Sem.Dyn.T Phi (S.eval_type t) -> *)
+ (*      T.Sem.Dyn.T (compile_state Phi) (T.eval_type (scheme t)) -> Type *)
 
+  Definition okdyn t : S.Sem.Dyn.T Phi (S.eval_type (t)) -> 
+                       T.Sem.Dyn.T (compile_state Phi) (T.eval_type (scheme t)) -> 
+                       Prop 
+  := fun dyn1 dyn2 => 
+  forall st1 st2, 
+             forall delta1 delta2, lr_diff _ delta1 delta2 -> 
+             dyn1 st1 delta1 = dyn2 st2 delta2. 
+                                 
+  
+
+  Definition ok t a1 a2 :=
+    okdyn t (S.Sem.eval_action a1) (T.Sem.eval_action (compile T.eval_type t a2)). 
+  
+  Definition Denote Phi t (e : T.Action Phi t ) := T.Sem.eval_action (e _).   
+
+  Definition Ok t a := okdyn _ _ (Denote (compile_state Phi) t a).  
+  
+  Notation "B '/' Delta" := (S.Sem.eval_action B Delta) (at level 60, no associativity). 
+  Notation "B '/' Delta" := (S.Sem.eval_action B Delta) (at level 60, no associativity). 
+  Lemma correct t a Delta :  C t a /s Delta = Delta. 
+
+End t.
+
+
+
+(* Class Ordered  (X : Type) := {compare : X -> X -> comparison}.   *)
+
+(* Local Notation lex e f := (match e with Eq => f | _ => e end). *)
+
+
+(* Module M.  *)
+  
+(*   Section t.  *)
+(*     Variable X : Type.  *)
+(*     Context {O : Ordered X}.  *)
     
-  Qed.     
     
-  
-  Definition compile_expr t : S.expr (fun x => R (flat x)) t  -> T.expr R (flat t).  
 
-  refine (let compile := fix compile t (e : S.expr (fun x => R (flat x)) t) : T.expr R (flat t) := 
-              match e with
-                | S.Evar t v => T.Evar v
-                | S.Ebuiltin args res f x => _
-                | S.Econstant ty c => T.Econstant c
-                | S.Efst l t x => T.Efst _ _ _ (compile _ x)
-                | S.Esnd l t x => T.Esnd _ _ _ (compile _ x)
-                | S.Enth l t m x => T.Enth  (var_map _ _ _ m) (compile _ x) 
-                | S.Etuple l exprs => T.Etuple _ _ _ 
-                | S.Econstr l t c x => _
-
-              end  
-          in compile t
-         ). 
-  eapply (T.Ebuiltin f). eapply DList.dlist_map.  2: apply x. 
-  simpl. intros. apply (compile (S.Tlift x0) X).    
- 
-   Definition zob {A B} (F : A -> Type) (G: B -> Type) (C : A -> B) (D : forall x, F x -> G ( C x)) (l: list  A) (dl : DList.dlist F l) : DList.dlist G (List.map C l). 
-  induction dl. simpl. constructor. 
-  simpl. constructor. apply D.  auto. 
-  apply IHdl. 
-  Defined. 
-  
-  
-  
-  eapply (zob _ _ _ compile) in exprs. apply exprs.
-  apply (allocate _ _ c (compile _ x)). 
-  Defined. 
-
-
-  Definition compile   t : S.action Phi (fun x => R (flat x )) t -> T.action (compile_state Phi ) R (flat t). 
-  refine (let compile := fix compile t (a : S.action Phi (fun x => R (flat x)) t) : 
-              T.action (compile_state Phi) R (flat t) :=
-              match a with
-                | S.Return t exp => T.Return (compile_expr _ exp)
-                | S.Bind t u a f => T.Bind (compile _ a) (fun X => compile _ (f X))  
-                | S.Assert e => T.Assert (compile_expr _ e)
-                | S.Primitive args res p exprs => 
-                    let exprs := 
-                        (zob (S.expr (fun x : S.type => R (flat x))) 
-                             (T.expr R) flat compile_expr args exprs)
-                    in 
-                      T.Primitive (List.map flat args) (flat res) _ exprs
-                | S.Try a => T.Try _ _ (compile _ a)
-                | S.Case td l t c e x => _
-              end
-          in compile t
-         ). 
-  clear exprs0. revert exprs. 
-  refine (match p with 
-              S.register_read t v => fun exprs =>
-                                     (
-                                       T.register_read  (var_map compile_sync _ _ v)
-                                       :T.primitive (compile_state Phi) (List.map flat []) (flat t))
-              
-            | S.register_write t v => fun exprs => 
-                                     (
-                                       T.register_write (var_map compile_sync Phi (S.Treg t) v)
-                                       :T.primitive (compile_state Phi) (List.map flat [t])
-                                         (flat (S.Tlift Tunit))
-                                     )
-            | S.regfile_read n t v p => fun exprs => ( T.regfile_read
-                                                      (var_map compile_sync Phi (S.Tregfile n t) v) p
-                                                     :T.primitive (compile_state Phi)
-                                                       (List.map flat [S.Tlift (W p)]) 
-                                                       (flat t))
-            | S.regfile_write m t v p => fun exprs => 
-
-                                          (   T.regfile_write
-                   (var_map compile_sync Phi (S.Tregfile m t) v) p
-                 :T.primitive (compile_state Phi)
-                    (List.map flat [S.Tlift (W p); t])
-                    (flat (S.Tlift Tunit)))
-         end ). 
-  (* Case case *)
-  + apply compile_expr in e.
-    Import T. 
-    refine (T.Bind (T.Assert _) (fun _ => _)). 
-    refine (_  = _ )%expr. 
-    eapply Econstant. exact (fin_of_var _ _ c : constant0 (Tfin _)). 
-    simpl in e. apply Efst in e. apply e. 
+(*     Definition T := list (positive * X).  *)
     
-    clear _H. set (y := fun e => compile _ (x e)). clearbody y. clear x.  clear - e y c. 
-   apply (deallocate _ _ _ c e y). 
-  
-  Defined. 
+(*     Definition singleton x : T := ([(1%positive,x)])%list.  *)
+    
+(*     Fixpoint add n x (l : T) : T := *)
+(*       match l with  *)
+(*         | nil => [(n,x)] *)
+(*         | (m,y)::q =>  *)
+(*             match compare x y with  *)
+(*               | Lt => (n, x) :: l *)
+(*               | Eq => (n+m,x)%positive :: q  *)
+(*               | Gt => (m,y):: add n x q *)
+(*             end *)
+(*       end%list.  *)
+
+(*     Fixpoint max n x (l : T) : T := *)
+(*       match l with  *)
+(*         | nil => [(n,x)] *)
+(*         | (m,y)::q =>  *)
+(*             match compare x y with  *)
+(*               | Lt => (n, x) :: l *)
+(*               | Eq => (Pos.max n m,x)%positive :: q  *)
+(*               | Gt => (m,y):: max n x q *)
+(*             end *)
+(*       end%list.  *)
+    
+(*     Fixpoint union (a b : T) : T := *)
+(*       match a with  *)
+(*         |nil => b  *)
+(*         | (n,x) :: q => add n x (union q b) *)
+(*       end%list.  *)
+
+(*     Fixpoint join (a b : T) : T := *)
+(*       match a with  *)
+(*         |nil => b  *)
+(*         | (n,x) :: q => max n x (join q b) *)
+(*       end%list.  *)
+    
+(*     Fixpoint copy n (x : X)  := *)
+(*       match n with  *)
+(*         | xH => [x] *)
+(*         | xO m => copy m x ++ copy m x *)
+(*         | xI m => x :: copy m x  ++ copy m x *)
+(*       end%list.  *)
+
+(*     Fixpoint contents (a : T) :=  *)
+(*       match a with  *)
+(*         | nil => nil *)
+(*         | (n,x) :: q => copy n x ++ (contents q) *)
+(*       end%list.          *)
+    
+(*     Fixpoint elements (a : T) : list X := List.map (@snd _ _) a.  *)
+    
+(*     Fixpoint of_list (l : list X) : T := *)
+(*       match l with  *)
+(*         | nil => nil *)
+(*         | cons t q => add 1 t (of_list q) *)
+(*       end.  *)
+(*   End t.  *)
+(*   Arguments singleton {X} _.  *)
+(*   Arguments add {X _} n x l.  *)
+(*   Arguments union {X _} a b.  *)
+(*   Arguments join {X _} a b.  *)
+(*   Arguments of_list {X _} l.   *)
+
+(* End M.  *)
+
+(* Definition type0_cmp t t' :=  *)
+(*   match t , t' with  *)
+(*     | Tunit, Tunit => Eq *)
+(*     | Tbool, Tbool => Eq *)
+(*     | Tint n , Tint m => NPeano.Nat.compare n m  *)
+(*     | Tfin n , Tfin m => NPeano.Nat.compare n m  *)
+
+(*     | Tunit, _ => Lt *)
+(*     | _, Tunit => Gt *)
+
+(*     | Tbool, _ => Lt *)
+(*     | _, Tbool => Gt *)
+
+(*     | Tint _, _ => Lt *)
+(*     | _, Tint _ => Gt *)
+
+(*     | Tfin _, _ => Lt *)
+(*     | _, Tfin _ => Gt        *)
+
+(*     | Tabstract _ _, _ => Lt *)
+(*   end.  *)
+
+(* Fixpoint type_cmp  t t' {struct t} := *)
+(*   match t, t' with  *)
+(*       | T.Tlift t, T.Tlift t' => type0_cmp t t' *)
+(*       | T.Ttuple l, T.Ttuple l' =>  *)
+(*           let list_compare := fix list_compare h k := *)
+(*               match h,k with  *)
+(*                 | nil, nil => Eq *)
+(*                 | nil, _ => Lt *)
+(*                 | _, nil => Gt *)
+(*                 | cons t q, cons t' q' => lex (type_cmp t t') (list_compare q q') *)
+(*               end in  *)
+
+(*           list_compare l l'  *)
+(*       | T.Tlift _, _ => Lt *)
+(*       | _,  T.Tlift _ => Gt *)
+(*   end.  *)
